

$$\begin{aligned}
 &= \frac{1}{\pi} \left[\int_{-\pi}^0 (x+\pi) \sin nx dx + \int_0^{\pi} (x+\pi) \sin nx dx \right] \\
 &= \frac{1}{\pi} \left[-\frac{(x+\pi)}{n} \cos nx + \frac{1}{n} \sin nx \right]_{-\pi}^0 + \frac{1}{\pi} \left[-\frac{(x+\pi)}{n} \cos nx + \frac{1}{n} \sin nx \right]_0^{\pi} \\
 &= \frac{1}{\pi} \left[\left(\frac{\pi}{n} + 0 \right) - (0 - 0) \right] + \frac{1}{\pi} \left[\left(-\frac{2\pi}{n} (-1)^n + 0 \right) - \left(-\frac{\pi}{n} (1) + 0 \right) \right] \\
 &= \frac{1}{\pi} \left[\frac{\pi}{n} - \frac{2\pi}{n} (-1)^n + \frac{\pi}{n} \right] \\
 &= \frac{2}{n} [1 - (-1)^n]
 \end{aligned}$$

$$\therefore \text{F.S} \Rightarrow f(x) = \frac{\pi}{2} + \sum_{n=1}^{\infty} \left[\frac{2((-1)^n - 1) \cos nx}{\pi n^2} + \frac{2[1 - (-1)^n] \sin nx}{n} \right]$$

Q.3 Obtain F.S for $f(x) = \begin{cases} x + \pi/2, & -\pi < x < 0 \\ \pi/2 - x, & 0 < x < \pi \end{cases}$

Hence deduce that, i) $\frac{\pi^2}{8} = \frac{1}{1^2} + \frac{1}{3^2} + \frac{1}{5^2} + \dots$ ii) $\frac{\pi^4}{96} = \frac{1}{1^4} + \frac{1}{3^4} + \frac{1}{5^4} + \dots$

* Parseval Identity for $f(x)$ in $(-\pi, \pi)$:-

If $f(x)$ converges uniformly in open interval $-\pi$ to π , then F.S for $f(x)$ is given by -

$$f(x) = a_0 + \sum_{n=1}^{\infty} (a_n \cos nx + b_n \sin nx)$$

And Parseval's Identity in $(-\pi, \pi)$ is given by -

$$\frac{1}{2\pi} \int_{-\pi}^{\pi} [f(x)]^2 dx = a_0^2 + \frac{1}{2} \sum_{n=1}^{\infty} [a_n^2 + b_n^2]$$

$$\Rightarrow f(-x) = \begin{cases} -x + \pi/2, & -\pi < -x < 0 \\ \pi/2 - (-x), & 0 < x < \pi \end{cases}$$

$$f(-x) = \begin{cases} \pi/2 - x, & \pi > x > 0 \\ \pi/2 + x, & 0 > x > -\pi \end{cases}$$

$$f(-x) = f(x)$$

\therefore It is an even funⁿ.

$$\therefore b_n = 0$$

$$\text{now, } a_0 = \frac{1}{2\pi} \int_{-\pi}^{\pi} f(x) dx$$

$$= \frac{1}{\pi} \int_0^{\pi} f(x) dx$$

$$= \frac{1}{\pi} \int_0^{\pi} \left(\frac{\pi}{2} - x\right) dx$$

$$= \frac{1}{\pi} \left[\frac{\pi x}{2} - \frac{x^2}{2} \right]_0^{\pi}$$

$$= \frac{1}{2\pi} [(\pi^2 - \pi^2) - (0 - 0)]$$

$$= 0$$

$$a_n = \frac{1}{\pi} \int_{-\pi}^{\pi} f(x) \cos nx dx$$

$$= \frac{2}{\pi} \int_0^{\pi} f(x) \cos nx dx$$

$$= \frac{2}{\pi} \int_0^{\pi} (\pi/2 - x) \cos nx dx$$

$$= \frac{2}{\pi} \left[\left(\frac{\pi}{2} - x\right) \left(\frac{\sin nx}{n}\right) - (-1) \left(-\frac{\cos nx}{n^2}\right) \right]_0^{\pi}$$

$$= \frac{2}{\pi} \left[\left(0 - \frac{(-1)^n}{n^2} \right) - \left(0 - \frac{1}{n^2} \right) \right]$$

$$= \frac{2}{\pi n^2} [1 - (-1)^n]$$

∴ Fourier series \Rightarrow

$$f(x) = \sum_{n=1}^{\infty} \frac{2}{\pi n^2} [1 - (-1)^n] \sin nx$$

now, at $x=0$, fun is discontinuous.

$$f(0) = \frac{1}{2} \left[\lim_{x \rightarrow 0^-} f(x) + \lim_{x \rightarrow 0^+} f(x) \right]$$

$$= \frac{1}{2} \left[\frac{\pi}{2} + \frac{\pi}{2} \right]$$

$$= \frac{\pi}{2}$$

For deduction, put $x=0$ in F.S

$$\therefore f(0) = \sum_{n=1}^{\infty} \frac{2}{\pi n^2} [1 - (-1)^n] \sin(0)$$

$$\therefore \frac{\pi}{2} = \frac{2}{\pi} \sum_{n=1}^{\infty} \frac{(1 - (-1)^n)}{n^2}$$

$$\therefore \frac{\pi^2}{4} = \frac{2}{1^2} + \frac{2}{3^2} + \frac{2}{5^2} + \dots$$

$$\therefore \frac{\pi^2}{8} = \frac{1}{1^2} + \frac{1}{3^2} + \frac{1}{5^2} + \dots$$

Hence Proved.

$$\text{now, To deduce, } \frac{\pi^4}{96} = \frac{1}{1^4} + \frac{1}{3^4} + \frac{1}{5^4} + \dots$$

we need to use Parseval's Identity.

$$\frac{1}{2\pi} \int_{-\pi}^{\pi} [f(x)]^2 dx = a_0^2 + \frac{1}{2} \sum_{n=1}^{\infty} [a_n^2 + b_n^2] \quad \dots \text{Parseval's Identity}$$

$$= \frac{1}{2\pi} \int_{-\pi}^{\pi} [f(x)]^2 dx = \frac{1}{2} \sum_{n=1}^{\infty} \left(\frac{2}{\pi n^2} [1 - (-1)^n] \right)^2$$

$$= \frac{1}{\pi} \int_0^{\pi} [f(x)]^2 dx = \frac{1}{2} \times \frac{4}{\pi^2} \sum_{n=1}^{\infty} \frac{[1 - (-1)^n]^2}{n^4}$$

$$= \frac{1}{\pi} \int_0^{\pi} \left(\frac{\pi - x}{2} \right)^2 dx = \frac{2}{\pi^2} \left[\frac{4}{4^4} + \frac{4}{3^4} + \frac{4}{5^4} + \dots \right]$$

$$\frac{1}{\pi} \left[\frac{1}{3} \left(\frac{\pi - x}{2} \right)^3 \right]_0^{\pi} = \frac{8}{\pi^2} \left[\frac{1}{1^4} + \frac{1}{3^4} + \frac{1}{5^4} + \dots \right]$$

$$\frac{1}{\pi} \times \frac{-1}{3} \left[\left(\frac{-\pi}{2} \right)^3 - \left(\frac{\pi}{2} \right)^3 \right] = \frac{8}{\pi^2} \left[\frac{1}{1^4} + \frac{1}{3^4} + \frac{1}{5^4} + \dots \right]$$

$$\frac{-1}{3\pi} \left[-\frac{2\pi^3}{8} \right] = \frac{8}{\pi^2} \left[\frac{1}{1^4} + \frac{1}{3^4} + \frac{1}{5^4} + \dots \right]$$

$$\therefore \frac{\pi^4}{96} = \frac{1}{1^4} + \frac{1}{3^4} + \frac{1}{5^4} + \dots$$

hence proved.

H.W

Q. Find Fourier Series of $f(x) = \begin{cases} -\pi, & -\pi < x < 0 \\ x, & 0 < x < \pi \end{cases}$

hence deduce that, $\sum_{n=1}^{\infty} \frac{1}{(2n-1)^2} = \frac{\pi^2}{8}$

* Fourier series in $(c, c+2l)$:

Form of FS in $(c, c+2l)$ i.e. in $(0, 2l)$ or $(-l, l)$

$$f(x) = a_0 + \sum_{n=1}^{\infty} \left[a_n \cos\left(\frac{n\pi x}{l}\right) + b_n \sin\left(\frac{n\pi x}{l}\right) \right]$$

For interval in $(0, 2l)$:

$$a_0 = \frac{1}{2l} \int_0^{2l} f(x) dx$$

$$a_n = \frac{1}{l} \int_0^{2l} f(x) \cos\left(\frac{n\pi x}{l}\right) dx$$

$$b_n = \frac{1}{l} \int_0^{2l} f(x) \sin\left(\frac{n\pi x}{l}\right) dx$$

For interval in $(-l, l)$:

$$a_0 = \frac{1}{2l} \int_{-l}^l f(x) dx$$

$$a_n = \frac{1}{l} \int_{-l}^l f(x) \cos\left(\frac{n\pi x}{l}\right) dx$$

$$b_n = \frac{1}{l} \int_{-l}^l f(x) \sin\left(\frac{n\pi x}{l}\right) dx$$

* Parseval's identity in $f(x)$ in interval $(c, c+2l)$:

$$\frac{1}{2l} \int_c^{c+2l} [f(x)]^2 dx = a_0^2 + \frac{1}{2} \sum_{n=1}^{\infty} [a_n^2 + b_n^2]$$

* Parseval's identity in $(0 \text{ to } 2l)$:

$$\frac{1}{2l} \int_0^{2l} [f(x)]^2 dx = a_0^2 + \frac{1}{2} \sum_{n=1}^{\infty} [a_n^2 + b_n^2]$$

* Parseval's identity in $(-l \text{ to } l)$:

$$\frac{1}{2l} \int_{-l}^l [f(x)]^2 dx = a_0^2 + \frac{1}{2} \sum_{n=1}^{\infty} [a_n^2 + b_n^2]$$

Q.7 Find FS for $f(x) = \begin{cases} \pi x, & 0 \leq x \leq 1 \\ \pi(2-x), & 1 \leq x \leq 2 \end{cases}$ with period 2.

Hence deduce that, $\frac{\pi^2}{8} = \frac{1}{1^2} + \frac{1}{3^2} + \frac{1}{5^2} + \dots$

here, $l=1$

$\therefore F.S \Rightarrow$

$$f(x) = a_0 + \sum_{n=1}^{\infty} [a_n \cos(n\pi x) + b_n \sin(n\pi x)]$$

$$a_0 = \frac{1}{2l} \int_0^2 f(x) dx$$

$$= \frac{1}{2} \left[\int_0^1 \pi x dx + \int_1^2 \pi(2-x) dx \right]$$

$$= \frac{1}{2} \left[\left. \frac{\pi x^2}{2} \right|_0^1 + \left. \pi(2x - \frac{x^2}{2}) \right|_1^2 \right]$$

$$= \frac{1}{2} \left[\left(\frac{\pi}{2} - 0 \right) + \pi \left((4 - \frac{4}{2}) - (2 - \frac{1}{2}) \right) \right]$$

$$= \frac{1}{2} \left[\frac{\pi}{2} + \pi \left(2 - \frac{3}{2} \right) \right]$$

$$= \frac{1}{2} \left[\frac{\pi}{2} + \frac{\pi}{2} \right]$$

$$= \frac{\pi}{2}$$

$$a_n = \frac{1}{l} \int_0^2 f(x) \cos(n\pi x) dx$$

$$= \int_0^1 \pi x \cos n\pi x dx + \int_1^2 \pi(2-x) \cos n\pi x dx$$

$$= \left[\frac{\pi x (\sin n\pi x)}{n\pi} - (\pi) \left(\frac{-\cos n\pi x}{(n\pi)^2} \right) \right]_0^1 + \left[\frac{\pi(2-x) \sin n\pi x}{n\pi} - \right.$$

$$\left. \frac{\pi \left(\frac{-\cos n\pi x}{(n\pi)^2} \right)}{n\pi} \right]_1^2$$

$$= \left[\left(\frac{1}{n} \sin n\pi + \frac{1}{n^2\pi} \cos n\pi \right) - \left(0 + \frac{1}{n^2\pi} \cos 0 \right) \right] +$$

$$\left[\left(0 + \frac{1}{n^2\pi} \cos 2\pi \right) - \left(\frac{1}{n} \sin n\pi + \frac{1}{n^2\pi} \cos n\pi \right) \right]$$

$$= \left[\left(0 + \frac{1}{n^2\pi} (-1)^n \right) - \left(\frac{1}{n^2\pi} \right) + \left(\frac{1}{n^2\pi} \right) + \left(0 + \frac{1}{n^2\pi} (-1)^n \right) \right]$$

$$= \frac{2}{n^2\pi} [(-1)^n - 1]$$

$$b_n = \frac{1}{[0]_0} \int_0^2 f(x) \sin(n\pi x) dx$$

$$= \int_0^1 \pi x \sin n\pi x dx + \int_1^2 \pi(2-x) \sin n\pi x dx$$

$$= \left[\pi x \left(\frac{-\cos n\pi x}{n\pi} \right) - (\pi) \left(\frac{-\sin n\pi x}{(n\pi)^2} \right) \right]_0^1 +$$

$$\left[\pi(2-x) \left(\frac{-\cos n\pi x}{n\pi} \right) - (-\pi) \left(\frac{-\sin n\pi x}{(n\pi)^2} \right) \right]_1^2$$

$$= \left[\left(-\frac{1}{n} \cos n\pi + \frac{1}{n^2\pi} \sin n\pi \right) - \left(0 + \frac{1}{n^2\pi} \sin 0 \right) \right] +$$

$$\left[\left(0 - \frac{1}{n^2\pi} \sin 2n\pi \right) - \left(-\frac{1}{n} \cos n\pi - \frac{1}{n^2\pi} \sin n\pi \right) \right]$$

$$= \left[-\frac{(-1)^n}{n} + 0 - 0 + 0 + \frac{(-1)^n}{n} + 0 \right]$$

$$= 0$$

$$\therefore \text{F.S.} \Rightarrow f(x) = \frac{\pi}{2} + \sum_{n=1}^{\infty} \left[\frac{2[(-1)^n - 1]}{n^2\pi} \cos n\pi x \right]$$

now,

$$\pi x = \frac{\pi}{2} + \sum_{n=1}^{\infty} \frac{2}{n^2\pi} [(-1)^n - 1] \cos n\pi x$$

for deduction, put $x=0$

$$\therefore 0 = \frac{\pi}{2} + \sum_{n=1}^{\infty} \frac{2}{n^2\pi} [(-1)^n - 1]$$

$$-\frac{\pi}{2} = \frac{2}{\pi} \left[\frac{-2}{(1)^2} + 0 - \frac{2}{(3)^2} + 0 - \frac{2}{(5)^2} + \dots \right]$$

$$-\frac{\pi}{4} = -2 \left[\frac{1}{(1)^2} + \frac{1}{(3)^2} + \frac{1}{(5)^2} + \frac{1}{(7)^2} + \dots \right]$$

$$\Rightarrow \frac{\pi}{8} = \frac{1}{1^2} + \frac{1}{3^2} + \frac{1}{5^2} + \dots \quad \text{Hence Proved.}$$



Q.3 Obtain FS for $f(x) = 2x - x^2$ in $(0, 3)$ and hence deduce that $\frac{1}{1^2} - \frac{1}{2^2} + \frac{1}{3^2} - \frac{1}{4^2} + \dots = \frac{\pi^2}{12}$.

\Rightarrow here, $l = \frac{3}{2}$.

$$\text{So, let } f(x) = a_0 + \sum_{n=1}^{\infty} \left[a_n \cos\left(\frac{2n\pi x}{3}\right) + b_n \sin\left(\frac{2n\pi x}{3}\right) \right]$$

$$a_0 = \frac{1}{2(3/2)} \int_0^3 (2x - x^2) dx$$

$$= \frac{1}{3} \int_0^3 \left[\frac{2x^2}{2} - \frac{x^3}{3} \right]_0^3$$

$$= \frac{1}{3} \left[\left(9 - \frac{27}{3} \right) - (0 - 0) \right]$$

$$= \frac{1}{3} \left[-\frac{5}{4} \right]$$

$$= -\frac{5}{12}, 0$$

$$a_n = \frac{1}{3/2} \int_0^3 (2x - x^2) \cos\left(\frac{2n\pi x}{3}\right) dx$$

$$= \frac{2}{3} \left[\frac{(2x - x^2) \sin\left(\frac{2n\pi x}{3}\right) - (2 - 2x) \left[-\cos\left(\frac{2n\pi x}{3}\right) \right]}{\left(\frac{2n\pi}{3}\right)^2} \right]$$

$$+ (-2) \left[\frac{-\sin\left(\frac{2n\pi x}{3}\right)}{\left(\frac{2n\pi}{3}\right)^3} \right]_0^3$$

$$= \frac{2}{3} \left[\frac{(-3) \sin 2n\pi}{2n\pi/3} + \frac{(-4) \cos 2n\pi}{(2n\pi/3)^2} + \frac{(2) \sin 2n\pi}{(2n\pi/3)^3} \right] =$$

$$\left[0 + \frac{(-4) \cos 0}{(2n\pi/3)^2} + 0 \right]$$

$$= \frac{2}{3} \left[\frac{-\cancel{4}x^3(1)}{4h^2\pi^2} - \frac{\cancel{4}x^3(1)}{4h^2\pi^2} \right]$$

$$= \frac{2}{3} \left[\frac{-\cancel{4}x^3}{4h^2\pi^2} \right] = \frac{2}{3} \left[\frac{-9}{h^2\pi^2} - \frac{9}{4h^2\pi^2} \right]$$

$$= \frac{-9}{3h^2\pi^2} = \frac{2}{3} \left[-\frac{3}{2} \left[\frac{9}{h^2\pi^2} \right] \right] = \frac{-9}{h^2\pi^2}$$

$$b_n = \frac{1}{3/2} \int_0^3 (2x - x^2) \sin\left(\frac{2n\pi x}{3}\right) dx$$

$$= \frac{2}{3} \left[(2x - x^2) \left(\frac{-\cos\left(\frac{2n\pi x}{3}\right)}{\frac{2n\pi}{3}} \right) - (2 - 2x) \left(\frac{-\sin\left(\frac{2n\pi x}{3}\right)}{\left(\frac{2n\pi}{3}\right)^2} \right) \right.$$

$$\left. + (-2) \left(\frac{\cos\left(\frac{2n\pi x}{3}\right)}{\left(\frac{2n\pi}{3}\right)^3} \right) \right]_0^3$$

$$= \frac{2}{3} \left[\frac{3 \cdot \cos 2n\pi}{2n\pi/3} + \frac{(-4) \sin 2n\pi}{\left(\frac{2n\pi}{3}\right)^2} + \frac{(-2) \cos 2n\pi}{\left(\frac{2n\pi}{3}\right)^3} \right] -$$

$$\left[0 + \frac{(2) \sin 0}{\left(\frac{2n\pi}{3}\right)^2} + \frac{(-2) \cos 0}{\left(\frac{2n\pi}{3}\right)^3} \right]$$

$$= \frac{2}{3} \left[\frac{9}{2n\pi} + 0 - \frac{2}{\left(\frac{2n\pi}{3}\right)^3} - 0 + 0 + \frac{2}{\left(\frac{2n\pi}{3}\right)^3} \right]$$

$$= \frac{2}{3} \left[\frac{9}{2n\pi} \right]$$

$$= \frac{3}{n\pi}$$

$$\therefore f.s \Rightarrow f(x) = \sum_{n=1}^{\infty} \left[\frac{-9 \cos\left(\frac{2n\pi x}{3}\right)}{h^2\pi^2} + \frac{3 \sin\left(\frac{2n\pi x}{3}\right)}{h\pi} \right]$$

$$\text{let } x=0$$

$$\therefore 0 = \sum_{n=1}^{\infty} \frac{-9}{\pi^2} \cdot \frac{1}{h^2} (1)$$

$$\therefore \frac{-\pi^2}{9} = \frac{1}{1^2} + \frac{1}{2^2} + \frac{1}{3^2} + \frac{1}{4^2} + \dots$$

Put $x = \frac{3}{2}$

$$\left[2\left(\frac{3}{2}\right) - \left(\frac{3}{2}\right)^2\right] = \sum_{n=1}^{\infty} \left[\frac{-9}{n^2 \pi^2} \cos(n\pi) + \frac{3}{n\pi} \sin(n\pi) \right]$$

$$\left[3 - \frac{9}{4}\right] = -\frac{9}{\pi^2} \sum_{n=1}^{\infty} \frac{(-1)^n}{n^2}$$

$$\frac{1}{4} \times \frac{-\pi^2}{8} = -\frac{1}{1^2} + \frac{1}{2^2} - \frac{1}{3^2} + \frac{1}{4^2} - \dots$$

$$\frac{\pi^2}{12} = \frac{1}{1^2} - \frac{1}{2^2} + \frac{1}{3^2} - \frac{1}{4^2} + \dots$$

Q.3] Obtain F.S for $f(x) = |x|$, $-2 < x < 2$

Hence deduce that, $\sum_{n=1}^{\infty} \frac{1}{(2n-1)^2} = \frac{\pi^2}{8}$

→

Here, $l = 2$

$$\therefore \text{F.S} \Rightarrow |x| = a_0 + \sum_{n=1}^{\infty} \left[a_n \cos\left(\frac{n\pi x}{2}\right) + b_n \sin\left(\frac{n\pi x}{2}\right) \right]$$

here,

$$|-x| = x = |x|$$

⇒ $f(x) = |x|$ is an even funⁿ.

$$a_0 = \frac{1}{2l} \int_{-l}^l f(x) dx$$

$$= \frac{1}{4} \int_0^2 f(x) dx$$

$$= \frac{1}{4} \int_0^2 |x| dx$$

$$= \frac{1}{4} \left[\frac{x^2}{2} \right]_0^2$$

$$= 1$$

$$a_n = \frac{1}{2} \int_{-1}^1 f(x) \cos\left(\frac{n\pi x}{2}\right) dx$$

$$= \frac{2}{2} \int_0^1 f(x) \cos\left(\frac{n\pi x}{2}\right) dx$$

$$= \frac{2}{2} \int_0^2 |x| \cos\left(\frac{n\pi x}{2}\right) dx$$

$$= \frac{x^2}{2} \left[\frac{2 \sin\left(\frac{n\pi x}{2}\right)}{n\pi/2} - (1) \left(\frac{-\cos\left(\frac{n\pi x}{2}\right)}{\left(\frac{n\pi}{2}\right)^2} \right) \right]_0^2$$

$$= \frac{1}{2} (4 - 0) = \left[\frac{2 \sin n\pi}{n\pi/2} + \frac{\cos n\pi}{(n\pi/2)^2} \right] - \left[0 + \frac{\cos 0}{(n\pi/2)^2} \right]$$

$$= 2 \cdot \quad = 0 + \frac{4(-1)^n}{n^2\pi^2} - \frac{4(1)}{n^2\pi^2}$$

$$= \frac{4}{n^2\pi^2} [(-1)^n - 1]$$

\therefore Since $f(x)$ is even funⁿ

$$\therefore b_n = 0$$

$$F.S \Rightarrow |x| = 1 + \sum_{n=1}^{\infty} \frac{4}{n^2\pi^2} [(-1)^n - 1] \cos\left(\frac{n\pi x}{2}\right)$$

To deduce, put $x = 0$

$$0 = 1 + \sum_{n=1}^{\infty} \frac{4}{n^2\pi^2} [(-1)^n - 1] (1)$$

$$-1 \times \frac{\pi^2}{4} = \frac{-2}{1^2} + 0 \frac{-2}{3^2} + 0 \frac{-2}{5^2} + \dots$$

$$\frac{\pi^2}{8} = \frac{1}{1^2} + \frac{1}{3^2} + \frac{1}{5^2} + \frac{1}{7^2} + \dots$$

$$\therefore \sum_{n=1}^{\infty} \frac{1}{(2n-1)^2} = \frac{\pi^2}{8}$$

* Fourier Transform :-

In real life problems not all funⁿ/events are periodic in nature. Fourier Transform deals with such non periodic funⁿ & hence it is very useful in practical applications.

If a funⁿ $f(x)$ is defined in $(-\infty, \infty)$, is piecewise continuous in each finite interval & is absolutely integrable in $(-\infty, \infty)$ then integral $\frac{1}{\sqrt{2\pi}} \int_{-\infty}^{\infty} f(x) e^{isx} dx$ is called Fourier Transform of $f(x)$ & it is denoted by $F(s)$.

i.e.
$$F(s) = \frac{1}{\sqrt{2\pi}} \int_{-\infty}^{\infty} f(x) e^{isx} dx$$

eg. $f(x) = x^2, 0 < x < 2$

then,
$$F(s) = \frac{1}{\sqrt{2\pi}} \int_{-\infty}^{\infty} f(x) e^{isx} dx$$

$$= \frac{1}{\sqrt{2\pi}} \int_0^2 x^2 \cdot e^{isx} dx$$

* Fourier sine transform & cosine transform :-

If $f(x)$ is defined in $(0, \infty)$, we define its -

1) F.S.T by

$$F_s(s) = \sqrt{\frac{2}{\pi}} \int_0^{\infty} f(x) \sin sx dx$$

2) F.C.T by

$$F_c(s) = \sqrt{\frac{2}{\pi}} \int_0^{\infty} f(x) \cos sx dx$$

Q.1 Find the Fourier Transform of $f(x) = \begin{cases} 1+x/a, & -a < x < 0 \\ 1-x/a, & 0 < x < a \\ 0, & \text{otherwise} \end{cases}$

By definition,

$$\begin{aligned} F(s) &= \frac{1}{\sqrt{2\pi}} \int_{-\infty}^{\infty} f(x) e^{isx} dx \\ &= \frac{1}{\sqrt{2\pi}} \left[\int_{-a}^0 \left(1 + \frac{x}{a}\right) e^{isx} dx + \int_0^a \left(1 - \frac{x}{a}\right) e^{isx} dx \right] \\ &= \frac{1}{\sqrt{2\pi}} \left[\left(\left(1 + \frac{x}{a}\right) \frac{e^{isx}}{is} - \left(\frac{1}{a}\right) \left[\frac{e^{isx}}{(is)^2} \right] \right)_{-a}^0 + \left(\left(1 - \frac{x}{a}\right) \frac{e^{isx}}{is} - \left(-\frac{1}{a}\right) \left[\frac{e^{isx}}{(is)^2} \right] \right)_0^a \right] \\ &= \frac{1}{\sqrt{2\pi}} \left[\left(\frac{1}{is} - \frac{1}{a(is)^2} \right) - \left(0 - \frac{e^{-isa}}{a(is)^2} \right) + \left(0 + \frac{e^{isa}}{a(is)^2} \right) - \left(\frac{1}{is} + \frac{1}{a(is)^2} \right) \right] \\ &= \frac{1}{\sqrt{2\pi}} \left[\cancel{\frac{1}{is}} - \frac{1}{a(is)^2} + \frac{e^{-isa}}{a(is)^2} + \frac{e^{isa}}{a(is)^2} - \cancel{\frac{1}{is}} - \frac{1}{a(is)^2} \right] \\ &= \frac{1}{\sqrt{2\pi}} \left[\frac{2}{as^2} - \frac{e^{isa}}{as^2} - \frac{e^{-isa}}{as^2} \right] \\ &= \frac{1}{\sqrt{2\pi}} \left[\frac{2}{as^2} - \frac{1}{as^2} [\cos as + i \sin as + \cos as - i \sin as] \right] \\ &= \frac{1}{\sqrt{2\pi}} \left[\frac{2}{as^2} - \frac{2 \cos as}{as^2} \right] \\ &= \frac{\sqrt{2}}{\pi} \cdot \frac{1}{as^2} [1 - \cos as] \end{aligned}$$

Q.2 Find Fourier cosine transform of $f(x) = \begin{cases} \cos x, & 0 < x < a \\ 0, & x > a \end{cases}$

$$\star \left[\int_0^\infty \frac{\sin \theta}{\theta} d\theta = \frac{\pi}{2} \right] \text{ (imp)}$$

$$\begin{aligned}
 \Rightarrow F_s(f(x)) &= \sqrt{\frac{2}{\pi}} \int_0^\infty f(x) \sin sx \, dx \\
 &= \sqrt{\frac{2}{\pi}} \left[\int_0^a \cos x \sin sx \, dx + \int_a^\infty (0) \sin sx \, dx \right] \\
 &= \sqrt{\frac{2}{\pi}} \left[\int_0^a \frac{\cos sx \cos x}{2} \, dx \right] \\
 &= \frac{1}{\sqrt{2\pi}} \left[\int_0^a (\cos(s+x)x + \cos(s-x)x) \, dx \right] \\
 &= \frac{1}{\sqrt{2\pi}} \left[\frac{\sin(s+x)x}{(s+x)} + \frac{\sin(s-x)x}{(s-x)} \right]_0^a \\
 &= \frac{1}{\sqrt{2\pi}} \left[\frac{\sin(s+a)a}{(s+a)} + \frac{\sin(s-a)a}{(s-a)} - 0 - 0 \right] \\
 &= \frac{1}{\sqrt{2\pi}} \left[\frac{\sin(s+a)a}{(s+a)} + \frac{\sin(s-a)a}{(s-a)} \right]
 \end{aligned}$$

Q.3] Find Fourier sine transform of $\frac{1}{x}$.

\Rightarrow

$$\begin{aligned}
 F_s(f(x)) &= \sqrt{\frac{2}{\pi}} \int_0^\infty f(x) \sin sx \, dx \\
 &= \sqrt{\frac{2}{\pi}} \left[\int_0^\infty \frac{\sin sx}{x} \, dx \right]
 \end{aligned}$$

$$\text{Put } x = \frac{\theta}{s} \Rightarrow \frac{1}{x} = \frac{s}{\theta}$$

$$dx = \frac{1}{s} d\theta$$

$$= \sqrt{\frac{2}{\pi}} \left[\int_0^\infty \frac{s \sin \theta}{\theta} \cdot \frac{1}{s} d\theta \right]$$

$$= \sqrt{\frac{2}{\pi}} \times \frac{\pi}{2}$$

$$= \sqrt{\frac{\pi}{2}}$$

$$* \quad I = \int f(x, a) dx$$

$$\Rightarrow \frac{dI}{da} = \int \frac{\partial (f(x, a))}{\partial a} dx$$

$$\Rightarrow I = \int \text{Answer } da. \quad [\text{DUIS}]$$

* Q.47 Find the Fourier transform of $f(x) = e^{-x^2}$.
 \Rightarrow

$$\begin{aligned}
 F(s) &= \frac{1}{\sqrt{2\pi}} \int_{-\infty}^{\infty} f(x) e^{isx} dx \\
 &= \frac{1}{\sqrt{2\pi}} \int_{-\infty}^{\infty} \underbrace{e^{-x^2}}_{\text{even fun}} \cdot \underbrace{e^{isx}}_{\text{odd fun}} dx \\
 &= \frac{1}{\sqrt{2\pi}} \int_{-\infty}^{\infty} e^{-x^2} [\cos sx + i \sin sx] dx \\
 &= \frac{2}{\sqrt{2\pi}} \int_0^{\infty} e^{-x^2} \cos sx dx + 0
 \end{aligned}$$

$$\text{Let } I(s) = \int_0^{\infty} e^{-x^2} \cos sx dx$$

$$\begin{aligned}
 \frac{dI(s)}{ds} &= \int_0^{\infty} x \cdot e^{-x^2} \cdot (-\sin sx) dx \\
 &= -\frac{1}{2} \int_0^{\infty} \{e^{-x^2} (-2x)\} \sin sx dx
 \end{aligned}$$

$$\begin{array}{|l}
 \text{here, } \int e^{-x^2} (-2x) dx \\
 = e^{-x^2}
 \end{array}$$

$$= -\frac{1}{2} \left[\left(\sin sx (e^{-x^2}) \right)_0^{\infty} - \int_0^{\infty} s \cdot \cos sx \cdot e^{-x^2} dx \right]$$